Capybara/Syntax/Context/Core.lean
@@ -1,0 +1,123 @@
+import Mathlib.Data.Fin.Basic
+import Capybara.Syntax.Type
+namespace Capybara
+
+/-!
+Kind of a capture set parameter.
+-/
+inductive CKind : Nat -> Nat -> Type where
+| Sep : SepDegree n k -> CKind n k
+| Fresh : CKind n k
+
+/-!
+Type binding and capture set binding.
+
+Type binding can be either a type parameter (abstract) or
+a concrete type alias. Similarly, capture set binding can be
+a capture set parameter (abstract) or a concrete capture set alias.
+-/
+inductive TBinding : Nat -> Nat -> Nat -> Type where
+| param : SType n m k -> TBinding n m k
+| typealias : SType n m k -> TBinding n m k
+
+inductive CBinding : Nat -> Nat -> Type where
+| param : CKind n k -> CBinding n k
+| capturealias : CaptureSet n k -> CBinding n k
+
+notation:max "tparam" S => TBinding.param S
+notation:max "talias" S => TBinding.typealias S
+notation:max "cparam" k => CBinding.param k
+notation:max "calias" C => CBinding.capturealias C
+
+/-!
+Renaming functions for type and capture set binding.
+-/
+def CKind.rename : CKind n k -> Renaming n m k n' m' k' -> CKind n' k'
+| CKind.Sep D, ρ => CKind.Sep (D.rename ρ)
+| CKind.Fresh, _ => CKind.Fresh
+def TBinding.rename : TBinding n m k -> Renaming n m k n' m' k' -> TBinding n' m' k'
+| TBinding.param T, ρ => TBinding.param (T.rename ρ)
+| TBinding.typealias T, ρ => TBinding.typealias (T.rename ρ)
+def CBinding.rename : CBinding n k -> Renaming n m k n' m' k' -> CBinding n' k'
+| CBinding.param k, ρ => CBinding.param (k.rename ρ)
+| CBinding.capturealias C, ρ => CBinding.capturealias (C.rename ρ)
+
+/-!
+Weakening functions for type and capture set binding.
+-/
+def TBinding.weaken (B : TBinding n m k) : TBinding (n+1) m k :=
+  B.rename (Renaming.weaken)
+def CKind.weaken (K : CKind n k) : CKind (n+1) k :=
+  K.rename (Renaming.weaken (m:=0))
+def CBinding.weaken (B : CBinding n k) : CBinding (n+1) k :=
+  B.rename (Renaming.weaken (m:=0))
+def TBinding.tweaken (B : TBinding n m k) : TBinding n (m+1) k :=
+  B.rename (Renaming.tweaken)
+def TBinding.cweaken (B : TBinding n m k) : TBinding n m (k+1) :=
+  B.rename (Renaming.cweaken)
+def CKind.cweaken (K : CKind n k) : CKind n (k+1) :=
+  K.rename (Renaming.cweaken (m:=0))
+def CBinding.cweaken (B : CBinding n k) : CBinding n (k+1) :=
+  B.rename (Renaming.cweaken (m:=0))
+
+/-!
+An indexed context. A `Context n m k` contains `n` term variables,
+`m` type variables, and `k` capture set variables.
+!-/
+inductive Context : Nat -> Nat -> Nat -> Type where
+| empty : Context 0 0 0
+| cons : Context n m k -> CType n m k -> Context (n+1) m k
+| tcons : Context n m k -> TBinding n m k -> Context n (m+1) k
+| ccons : Context n m k -> CBinding n k -> Context n m (k+1)
+
+instance : EmptyCollection (Context 0 0 0) :=
+  ⟨Context.empty⟩
+
+theorem Context.empty_def :
+  ({} : Context 0 0 0) = Context.empty := rfl
+
+notation:20 Γ ",x:" T => Context.cons Γ T
+notation:20 Γ ",X:" T => Context.tcons Γ T
+notation:20 Γ ",c:" C => Context.ccons Γ C
+
+/-!
+Context lookup.
+
+`Context.Lookup`, `Context.LookupT`, and `Context.LookupC` look up the three dimensions of a context,
+respectively.
+-/
+inductive Context.Lookup : Context n m k -> Fin n -> CType n m k -> Prop where
+| here : Context.Lookup (Γ,x:T) 0 T.weaken
+| there :
+  Context.Lookup Γ x T ->
+  Context.Lookup (Γ,x:T) (x.succ) T.weaken
+| tthere :
+  Context.Lookup Γ x T ->
+  Context.Lookup (Γ,X:B) x (T.tweaken)
+| cthere :
+  Context.Lookup Γ x T ->
+  Context.Lookup (Γ,c:B) x (T.cweaken)
+inductive Context.LookupT : Context n m k -> Fin m -> TBinding n m k -> Prop where
+| here : Context.LookupT (Γ,X:T) 0 T.tweaken
+| there :
+  Context.LookupT Γ X S ->
+  Context.LookupT (Γ,x:T) X S.weaken
+| tthere :
+  Context.LookupT Γ X T ->
+  Context.LookupT (Γ,X:B) (X.succ) T.tweaken
+| cthere :
+  Context.LookupT Γ X T ->
+  Context.LookupT (Γ,c:B) X T.cweaken
+inductive Context.LookupC : Context n m k -> Fin k -> CBinding n k -> Prop where
+| here : Context.LookupC (Γ,c:C) 0 C.cweaken
+| there :
+  Context.LookupC Γ c C ->
+  Context.LookupC (Γ,x:T) c C.weaken
+| tthere :
+  Context.LookupC Γ c C ->
+  Context.LookupC (Γ,X:B) c C
+| cthere :
+  Context.LookupC Γ c C ->
+  Context.LookupC (Γ,c:B) (c.succ) C.cweaken
+
+end Capybara
